theories/logic/sem_sub_typing.v
@@ -78,6 +78,23 @@ Section sub_typing.
     iNext. by iApply Hκ₂₁.
   Qed.
 
+  (* Lemma sig_le_eff_rec (ι₁ ι₂ κ₁ κ₂ : sem_sig Σ -d> sem_ty Σ) *) 
+  (*   `{ NonExpansive ι₁, NonExpansive ι₂, NonExpansive κ₁, NonExpansive κ₂ } : *)
+  (*   (∀ ρ ρ', ρ ≤R ρ' → ι₁ ρ ≤T ι₂ ρ') → *)
+  (*   (∀ ρ ρ', ρ ≤R ρ' → κ₂ ρ' ≤T κ₁ ρ) → *)
+  (*   (μS: α, ι₁ α ⇒ κ₁ α) ≤R (μS: α, ι₂ α ⇒ κ₂ α). *)
+  (* Proof. *)
+  (*   iIntros (Hι₁₂ Hκ₂₁). iLöb as "IH". *)
+  (*   iIntros (v Φ) "!#". *) 
+  (*   rewrite !sem_sig_eff_rec_eq. *)
+  (*   iIntros "(%w & -> & Hι₁ & HκΦ₁)". *)
+  (*   iExists v; iSplitR; first done. *)
+  (*   iSplitL "Hι₁". *)
+  (*   { iNext. admit. iApply Hι₁₂. } *)
+  (*   iIntros (b) "Hκ₂". iApply "HκΦ₁". *)
+  (*   iNext. by iApply Hκ₂₁. *)
+  (* Qed. *)
+
   Lemma ty_le_refl (τ : sem_ty Σ) : τ ≤T τ.
   Proof. done. Qed.
   
